Add1sp1 memory safety and hints

code/mpfr/MPFR.Add1.Spec.fst
@@ -5,58 +5,64 @@ open MPFR.Dyadic
 open MPFR.Lib.Spec
 open MPFR.Maths
 
-#set-options "--z3refresh --z3rlimit 5 --max_fuel 1 --initial_fuel 0 --max_ifuel 1 --initial_ifuel 0"
+#set-options "--z3refresh --z3rlimit 15 --max_fuel 1 --initial_fuel 0 --max_ifuel 1 --initial_ifuel 0"
+
+(* In this specification we only consider MPFR normal numbers as input *)
 
 (* Useful functions when adding two MPFR numbers with same precision
  * and the exponent of the first one is greater than that of the second one *)
 val add_sp_ge_limb: a:mpfr_reg_fp -> b:mpfr_reg_fp -> Pure nat
     (requires (a.sign = b.sign /\ a.prec = b.prec /\ a.exp >= b.exp))
-    (ensures  (fun rm -> rm = abs (eval a +. eval b).significand /\
+    (ensures  (fun rm -> rm * a.sign = (eval a +. eval b).significand /\
                       rm % pow2 (a.len - a.prec) = 0))
     
 let add_sp_ge_limb a b =
-    lemma_distr_add_right a.sign (a.limb * pow2 (a.exp - b.exp)) (b.limb * pow2 0);
+    lemma_distr_add_left a.sign (a.limb * pow2 (a.exp - b.exp)) (b.limb * pow2 0);
+    //! assert((a.limb * pow2 (a.exp - b.exp) + b.limb) * a.sign = (eval a +. eval b).significand);
     lemma_mul_mod a.limb (pow2 (a.exp - b.exp)) (pow2 (a.len - a.prec));
-    lemma_mod_distr (a.limb * pow2 (a.exp - b.exp)) b.limb (pow2 (a.len - a.prec));
+    lemma_mod_distr_zero (a.limb * pow2 (a.exp - b.exp)) b.limb (pow2 (a.len - a.prec));
+    //! assert((a.limb * pow2 (a.exp - b.exp) + b.limb) % pow2 (a.len - a.prec) = 0);
     a.limb * pow2 (a.exp - b.exp) + b.limb
-    
+
+val add_sp_ge_len: a:mpfr_reg_fp -> b:mpfr_reg_fp -> Pure pos
+    (requires (a.sign = b.sign /\ a.prec = b.prec /\ a.exp >= b.exp))
+    (ensures  (fun rl -> add_sp_ge_limb a b >= pow2 (rl - 1) /\
+                      add_sp_ge_limb a b < pow2 rl))
+
+let add_sp_ge_len a b =
+    let d = a.exp - b.exp in
+    if add_sp_ge_limb a b < pow2 (a.len + d) then begin
+	lemma_mul_le_right (pow2 d) (pow2 (a.len - 1)) a.limb;
+	lemma_pow2_mul (a.len - 1) d;
+	//! assert(pow2 (a.len - 1 + d) <= add_sp_ge_limb a b);
+	a.len + d
+    end else begin
+        lemma_mul_lt_right (pow2 d) a.limb (pow2 a.len);
+        lemma_pow2_mul a.len d;
+	lemma_pow2_le b.len (a.len + d);
+        lemma_pow2_double (a.len + d);
+	//! assert(add_sp_ge_limb a b < pow2 (a.len + d + 1));
+	a.len + d + 1
+    end
+
 val add_sp_ge_exp: a:mpfr_reg_fp -> b:mpfr_reg_fp -> Pure int
     (requires (a.sign = b.sign /\ a.prec = b.prec /\ a.exp >= b.exp))
-    (ensures  (fun rx -> rx - nb_of_bits (add_sp_ge_limb a b) = (eval a +. eval b).exponent))
+    (ensures  (fun rx -> rx - add_sp_ge_len a b = (eval a +. eval b).exponent))
 
 let add_sp_ge_exp a b =
-    let d = a.exp - b.exp in
-    if add_sp_ge_limb a b < pow2 (nb_of_bits a.limb + d) then begin 
-	lemma_mul_le_right (pow2 d) (pow2 (nb_of_bits a.limb - 1)) a.limb;
-	lemma_pow2_mul (nb_of_bits a.limb - 1) d;
-	//! assert(pow2 (nb_of_bits a.limb - 1 + d) <= add_sp_ge_limb a b);
-	lemma_log2_le (pow2 (nb_of_bits a.limb - 1 + d)) (add_sp_ge_limb a b);
-	//! assert(add_sp_ge_limb a b < pow2 (nb_of_bits a.limb + d));
-	lemma_log2_lt (add_sp_ge_limb a b) (nb_of_bits a.limb + d);
-        a.exp
-    end else begin
-	lemma_log2_le (pow2 (nb_of_bits a.limb + d)) (add_sp_ge_limb a b);
-	//! assert(pow2 (nb_of_bits a.limb + d) <= add_sp_ge_limb a b);
-        lemma_mul_lt_right (pow2 d) a.limb (pow2 (nb_of_bits a.limb));
-        lemma_pow2_mul (nb_of_bits a.limb) d;
-	lemma_pow2_le (nb_of_bits b.limb) (nb_of_bits a.limb + d);
-        lemma_pow2_double (nb_of_bits a.limb + d);
-	//! assert(add_sp_ge_limb a b < pow2 (nb_of_bits a.limb + d + 1));
-	lemma_log2_lt (add_sp_ge_limb a b) (nb_of_bits a.limb + d + 1);
-        a.exp + 1
-    end
+    if add_sp_ge_limb a b < pow2 (a.len + a.exp - b.exp) then a.exp else a.exp + 1
     
-val add_sp_ge_prec: a:mpfr_fp -> b:mpfr_fp -> Pure pos
+val add_sp_ge_prec: a:mpfr_reg_fp -> b:mpfr_reg_fp -> Pure pos
     (requires (a.sign = b.sign /\ a.prec = b.prec /\ a.exp >= b.exp))
-    (ensures  (fun rp -> nb_of_bits (add_sp_ge_limb a b) - rp = nb_of_bits a.limb - a.prec))
+    (ensures  (fun rp -> add_sp_ge_len a b - rp = a.len - a.prec))
     
-let add_sp_ge_prec a b = a.prec + add_sp_ge_exp a b - b.exp
+let add_sp_ge_prec a b = a.prec + add_sp_ge_len a b - a.len
 
 (* Addition for two MPFR numbers with same precision *)
-val add_sp: a:mpfr_fp -> b:mpfr_fp -> Pure ieee_fp
+val add_sp: a:mpfr_reg_fp -> b:mpfr_reg_fp -> Pure normal_fp
     (requires (a.sign = b.sign /\ a.prec = b.prec))
     (ensures  (fun r -> eval a +. eval b =. eval r))
     
 let add_sp a b = 
     let a, b = if a.exp >= b.exp then a, b else b, a in
-    mk_ieee a.sign (add_sp_ge_prec a b) (add_sp_ge_exp a b) (add_sp_ge_limb a b) (nb_of_bits (add_sp_ge_limb a b))
+    mk_normal a.sign (add_sp_ge_prec a b) (add_sp_ge_exp a b) (add_sp_ge_limb a b) (add_sp_ge_len a b) MPFR_NUM
