code/mpfr/MPFR.Round.Spec.fst
@@ -1,4 +1,4 @@
-module MPFR.Rounding.Spec
+module MPFR.Round.Spec
 
 open FStar.Mul
 open FStar.UInt
@@ -6,65 +6,76 @@ open MPFR.Dyadic
 open MPFR.Lib.Spec
 open MPFR.Maths
 
-#set-options "--z3refresh --z3rlimit 5 --max_fuel 1 --initial_fuel 0 --max_ifuel 1 --initial_ifuel 0"
+#set-options "--z3refresh --z3rlimit 40 --max_fuel 1 --initial_fuel 0 --max_ifuel 1 --initial_ifuel 0"
 
 (* ulp definition *)
-let ulp (a:ieee_fp) = unit_fp (a.exp - a.prec)
-let half_ulp (a:ieee_fp) = unit_fp (a.exp - a.prec - 1)
+let ulp_p (a:normal_fp) (p:pos) = unit_fp (a.exp - p)
 
-val add_one_ulp: a:ieee_fp ->
-    Tot (r:ieee_fp{r.prec = a.prec /\ fabs (eval r) =. fabs (eval a) +. ulp a})
+let ulp (a:normal_fp) = ulp_p a a.prec
+let ufp (a:normal_fp) = ulp_p a 1
+
+val add_one_ulp: a:normal_fp ->
+    Tot (r:normal_fp{r.prec = a.prec /\ fabs (eval r) =. fabs (eval a) +. ulp a})
     
 let add_one_ulp a =
     if a.limb + pow2 (a.len - a.prec) < pow2 a.len then begin
-        lemma_mod_distr a.limb (pow2 (a.len - a.prec)) (pow2 (a.len - a.prec));
-	lemma_log2_le (pow2 (a.len - 1)) (a.limb + pow2 (a.len - a.prec));
-	lemma_log2_lt (a.limb + pow2 (a.len - a.prec)) a.len;
+        lemma_pow2_mod (a.len - a.prec) (a.len - a.prec);
+        lemma_mod_distr_zero a.limb (pow2 (a.len - a.prec)) (pow2 (a.len - a.prec));
 	{a with limb = a.limb + pow2 (a.len - a.prec)}
     end else begin
         lemma_pow2_multiple_le a.limb a.len (a.len - a.prec);
+	//! assert(a.limb + pow2 (a.len - a.prec) <= pow2 a.len);
 	lemma_pow2_mul (a.len - 1) 1;
+	//! assert(pow2 a.len * pow2 0 = pow2 (a.len - 1) * pow2 1);
 	lemma_pow2_mod (a.len - 1) (a.len - a.prec);
+	//! assert(pow2 (a.len - 1) % pow2 (a.len - a.prec) = 0);
 	{a with limb = pow2 (a.len - 1); exp = a.exp + 1}
     end
 
 (* Increase precision *)
-val incr_prec: a:ieee_fp -> p:pos{p >= a.prec} ->
-    Tot (r:ieee_fp{r.prec = p /\ eval r =. eval a})
+val incr_prec: a:normal_fp -> p:pos{p >= a.prec} ->
+    Tot (r:normal_fp{r.prec = p /\ eval r =. eval a})
     
 let incr_prec a p =
-    if p > a.len then
+    if p > a.len then begin
+        lemma_pow2_mul_range a.limb (p - a.len) a.len;
         {a with prec = p; limb = a.limb * pow2 (p - a.len); len = p}
-    else begin
+    end else begin
         lemma_pow2_mod_mod a.limb (a.len - a.prec) (a.len - p);
         {a with prec = p}
     end
 
 (* Decrease precision, actually RNDZ *)
-val decr_prec: a:ieee_fp -> p:pos{p < a.prec} ->
-    Tot (r:ieee_fp{r.prec = p /\
+val decr_prec: a:normal_fp -> p:pos{p < a.prec} ->
+    Tot (r:normal_fp{r.prec = p /\
         fabs (eval r) <=. fabs (eval a) /\ fabs (eval a) <. fabs (eval r) +. ulp r})
 	
-let decr_prec a p = 
+let decr_prec a p =
+    lemma_pow2_div_range a.limb (a.len - p) a.len;
+    lemma_pow2_mul_range (a.limb / pow2 (a.len - p)) (a.len - p) p;
     lemma_pow2_le (a.len - p) (a.len - 1);
     lemma_multiple_mod (a.limb / pow2 (a.len - p)) (pow2 (a.len - p));
     {a with prec = p; limb = (a.limb / pow2 (a.len - p)) * pow2 (a.len - p)}
 
 (* Split mantissa into high part and low part in order to round it
  * No need to normalize low_mant as long as it has the same value *)
-val high_mant: a:ieee_fp -> p:pos{p < a.prec} ->
-    Tot (hm:ieee_fp{hm.prec = p /\
+val high_mant: a:normal_fp -> p:pos{p < a.prec} ->
+    Tot (hm:normal_fp{hm.prec = p /\
         fabs (eval hm) <=. fabs (eval a) /\ fabs (eval a) <. fabs (eval hm) +. ulp hm})
 	
 let high_mant a p = decr_prec a p
 
-val low_mant: a:ieee_fp -> p:pos{p < a.prec} -> Tot (lm:valid_struct{
-    fabs (eval lm) <. ulp (high_mant a p)  /\ eval lm +. eval (high_mant a p) =. eval a})
+val low_mant: a:normal_fp -> p:pos{p < a.prec} -> Tot (lm:valid_fp{
+    fabs (eval lm) <. ulp (high_mant a p) /\ eval lm +. eval (high_mant a p) =. eval a})
     
 let low_mant a p = 
-    if a.limb % pow2 (a.len - p) = 0 then ()
-    else lemma_log2_lt (a.limb % pow2 (a.len - p)) (a.len - p);
-    {a with limb = a.limb % pow2 (a.len - p)}
+    lemma_euclidean a.limb (pow2 (a.len - p));
+    if a.limb % pow2 (a.len - p) = 0 then begin
+        {a with limb = 0; flag = MPFR_ZERO}
+    end else begin
+        lemma_pow2_mod_mod a.limb (a.len - p) (a.len - a.prec);
+        {a with limb = a.limb % pow2 (a.len - p)}
+    end
     
 
 ////////////////////////////////////////////////////////////////////////////////////
@@ -76,8 +87,8 @@ let low_mant a p =
 //                   abs r  <=  abs a  <  abs r + ulp r                           //
 ////////////////////////////////////////////////////////////////////////////////////
 
-val rndz_def: a:ieee_fp -> p:pos{p < a.prec} ->
-    Tot (r:ieee_fp{r.prec = p /\
+val rndz_def: a:normal_fp -> p:pos{p < a.prec} ->
+    Tot (r:normal_fp{r.prec = p /\
         fabs (eval r) <=. fabs (eval a) /\ fabs (eval a) <. fabs (eval r) +. ulp r})
 	
 let rndz_def a p = high_mant a p
@@ -94,19 +105,20 @@ let rndz_def a p = high_mant a p
 //////////////////////////////////////////////////////////////////////////////////////
 
 (* RNDN definition *)
-let is_even (a:ieee_fp) = (nth #a.len a.limb (a.prec - 1) = false)
+let is_even (a:normal_fp) = (nth #a.len a.limb (a.prec - 1) = false)
 
-let rndn_def (a:ieee_fp) (p:pos{p < a.prec}): Tot (r:ieee_fp{r.prec = p}) =
+let rndn_def (a:normal_fp) (p:pos{p < a.prec}): Tot (r:normal_fp{r.prec = p}) =
     let high, low = high_mant a p, low_mant a p in
-    if ((fabs (eval low) <. half_ulp high) || (fabs (eval low) =. half_ulp high && is_even high))
+    if ((fabs (eval low) <. ulp_p high (p + 1)) ||
+        (fabs (eval low) =. ulp_p high (p + 1) && is_even high))
     then rndz_def a p
     else add_one_ulp (rndz_def a p)
 
 (* Definitions of round bit and sticky bit which are widely used to implement RNDN *)
-let rb_def (a:ieee_fp) (p:pos{p < a.prec}): Tot bool = nth #a.len a.limb p
-let sb_def (a:ieee_fp) (p:pos{p < a.prec}): Tot bool = (a.limb % pow2 (a.len - p - 1) <> 0)
+let rb_def (a:normal_fp) (p:pos{p < a.prec}): Tot bool = nth #a.len a.limb p
+let sb_def (a:normal_fp) (p:pos{p < a.prec}): Tot bool = (a.limb % pow2 (a.len - p - 1) <> 0)
 
-val rb_value_lemma: a:ieee_fp -> p:pos{p < a.prec} ->
+val rb_value_lemma: a:normal_fp -> p:pos{p < a.prec} ->
     Lemma (a.limb % pow2 (a.len - p) = a.limb % pow2 (a.len - p - 1) + (if rb_def a p then pow2 (a.len - p - 1) else 0))
 
 let rb_value_lemma a p =
@@ -115,9 +127,9 @@ let rb_value_lemma a p =
     lemma_pow2_mod_div a.limb (a.len - p) (a.len - p - 1);
     lemma_pow2_mod_mod a.limb (a.len - p) (a.len - p - 1)
 
-val rb_sb_lemma: a:ieee_fp -> p:pos{p < a.prec} -> Lemma (
+val rb_sb_lemma: a:normal_fp -> p:pos{p < a.prec} -> Lemma (
     let lm_fp = fabs (eval (low_mant a p)) in
-    let hulp  = half_ulp (high_mant a p) in
+    let hulp  = ulp_p (high_mant a p) (p + 1) in
     ((rb_def a p = false /\ sb_def a p = false) <==> (lm_fp =. zero_fp)) /\
     ((rb_def a p = false /\ sb_def a p = true ) <==> (lm_fp >. zero_fp /\ lm_fp <. hulp)) /\
     ((rb_def a p = true  /\ sb_def a p = false) <==> (lm_fp =. hulp)) /\
@@ -135,7 +147,7 @@ let rb_sb_lemma a p =
 	lemma_pow2_mul (a.len - p - 1) (p + 1)
     end
 
-val is_even_lemma: a:ieee_fp -> p:pos{p < a.prec} -> Lemma
+val is_even_lemma: a:normal_fp -> p:pos{p < a.prec} -> Lemma
     (is_even (high_mant a p) = (logand #a.len (high_mant a p).limb (pow2 (a.len - p)) = 0))
     
 let is_even_lemma a p = 
@@ -147,15 +159,18 @@ let is_even_lemma a p =
     else 
         nth_lemma (logand #a.len (high_mant a p).limb (pow2_n #a.len (a.len - p))) (zero a.len)
 	
-val rndn_spec: a:ieee_fp -> p:pos{p < a.prec} ->
-    Tot (r:ieee_fp{r = rndn_def a p})
+val rndn_spec: a:normal_fp -> p:pos{p < a.prec} ->
+    Tot (r:normal_fp{r = rndn_def a p})
     
 let rndn_spec a p =
+    let high, low = high_mant a p, low_mant a p in
     rb_sb_lemma a p;
     is_even_lemma a p;
     if rb_def a p = false || 
       (sb_def a p = false && logand #a.len (high_mant a p).limb (pow2 (a.len - p)) = 0)
     then begin
+        assert ((fabs (eval low) <. ulp_p high (p + 1)) ||
+                (fabs (eval low) =. ulp_p high (p + 1) && is_even high));
 	rndz_def a p
     end else begin
 	add_one_ulp (rndz_def a p)
